adding several problems on nat -> {bool,nat} sequences

theories/MuRec/RA_UNIV_HALT.v
@@ -19,23 +19,55 @@ Set Implicit Arguments.
 
 Local Notation "'⟦' f '⟧'" := (@ra_rel _ f) (at level 0).
 
+(* We build a primitive µ-recursive algorithm
+
+     ra_pr_univ : recalg 2
+
+   with two argument (n##k##ø)
+     - n encodes a finitary valuation nat -> nat
+     - k encodes a finite list of H10C constraints
+   
+   1) ra_pr_univ always terminates (it is primitive recursive)
+   2) ra_pr_univ outputs 0 iff the valuation n solves the equations k
+
+*)
+
+Definition ra_pr_univ := ra_h10c_eval.
+
+Theorem ra_pr_univ_pr : prim_rec ra_pr_univ.
+Proof. apply ra_h10c_eval_pr. Qed.
+
+Definition PRIMEREC_UNIV_PROBLEM := nat.
+Definition PRIMEREC_UNIV_MEETS_ZERO (n : PRIMEREC_UNIV_PROBLEM) := exists k, ⟦ra_pr_univ⟧ (k##n##vec_nil) 0.
+
 (* We build a universal µ-recusive algorithm of size 8708
 
       ra_univ : recalg 1
 
     which is just a particular µ-recursive algorithm. It is
     universal w.r.t. elementary Diophantine constraints 
-    as established in Reductions/H10C_RA_UNIV.v
+    as established in Reductions/H10C_SAT_to_RA_UNIV_HALT.v
 
     Basically, its termination predicate RA_UNIV_HALT 
     can simulate the solvability of any list of elementary 
     Diophantine constraints, making it undecidable *)
+
+Definition ra_univ := ra_min_univ ra_pr_univ.
+
+Definition RA_UNIV_PROBLEM := nat.
+Definition RA_UNIV_HALT (n : RA_UNIV_PROBLEM) : Prop := ex (⟦ra_univ⟧ (n##vec_nil)).
+Definition RA_UNIV_AD_HALT (n : RA_UNIV_PROBLEM) : Prop := ex (⟦ra_univ_ad⟧ (n##vec_nil)).
 
 (* Check ra_size ra_univ. *)
 (* Eval compute in ra_size ra_univ. *)
 (* Check ra_size ra_univ_ad. *)
 (* Eval compute in ra_size ra_univ_ad. *)
 
-Definition RA_UNIV_PROBLEM := nat.
-Definition RA_UNIV_HALT (n : RA_UNIV_PROBLEM) : Prop := ex (⟦ra_univ⟧ (n##vec_nil)).
-Definition RA_UNIV_AD_HALT (n : RA_UNIV_PROBLEM) : Prop := ex (⟦ra_univ_ad⟧ (n##vec_nil)).
+Definition PRIMESEQ_PROBLEM := { f : recalg 1 | prim_rec f }.
+Definition PRIMESEQ_MEETS_ZERO (P : PRIMESEQ_PROBLEM) := exists n, ⟦proj1_sig P⟧ (n##vec_nil) 0.
+
+Definition NATSEQ_PROBLEM := nat -> nat.
+Definition NATSEQ_MEETS_ZERO (f : NATSEQ_PROBLEM) : Prop := exists n, f n = 0.
+
+Definition BOOLSEQ_PROBLEM := nat -> bool.
+Definition BOOLSEQ_MEETS_TRUE (f : BOOLSEQ_PROBLEM) : Prop := exists n, f n = true.
