theories/MuRec/Reductions/H10C_SAT_to_RA_UNIV_HALT.v
@@ -9,12 +9,16 @@
 
 Require Import List.
 
+From Undecidability.Shared 
+  Require Import pos vec.
+
 From Undecidability.MuRec 
-  Require Import recalg ra_univ ra_univ_andrej.
+  Require Import recalg beta ra_univ ra_univ_andrej.
 
 Require Import Undecidability.MuRec.RA_UNIV_HALT.
 
-Require Import Undecidability.DiophantineConstraints.H10C.
+From Undecidability.DiophantineConstraints
+ Require Import H10C Util.h10c_utils.
 
 Require Import Undecidability.Synthetic.Undecidability.
 
@@ -38,23 +42,58 @@ Local Notation "'⟦' f '⟧'" := (@ra_rel _ f) (at level 0).
      * lc is an instance of the H10C problem, ie a list of 
        h10c constraints *)
 
-Definition H10C_RA_UNIV : list h10c -> RA_UNIV_PROBLEM.
+Definition H10C_PRIMEREC_UNIV : list h10c -> PRIMEREC_UNIV_PROBLEM.
 Proof.
   intros lc.
-  destruct (nat_h10lc_surj lc) as (k & Hk).
+  destruct (nat_h10lc_surj lc) as (k & _).
   exact k.
 Defined.
 
-Theorem H10C_SAT_RA_UNIV_HALT : H10C_SAT ⪯  RA_UNIV_HALT.
+Theorem H10C_SAT_PRIMEREC_UNIV_MEETS_ZERO : H10C_SAT ⪯  PRIMEREC_UNIV_MEETS_ZERO.
 Proof.
-  exists H10C_RA_UNIV; intros lc.
-  unfold H10C_RA_UNIV.
+  exists H10C_PRIMEREC_UNIV; intros lc.
+  unfold H10C_PRIMEREC_UNIV.
   destruct (nat_h10lc_surj lc) as (k & Hk).
-  symmetry; apply ra_univ_spec; auto.
+  split.
+  + intros (phi & Hphi).
+    destruct (beta_fun_inv (h10lc_bound lc) phi) as (n & Hn).
+    generalize (h10lc_bound_prop _ _ Hn); clear Hn; intros Hn.
+    exists n; unfold ra_pr_univ; rewrite ra_h10c_eval_spec; eauto.
+    intros; apply Hn; auto.
+  + intros (n & Hn).
+    exists (beta n).
+    revert Hn; apply ra_h10c_eval_spec; auto.
 Qed.
 
-Check H10C_SAT_RA_UNIV_HALT.
+Theorem PRIMEREC_UNIV_MEETS_ZERO_RA_UNIV_HALT : PRIMEREC_UNIV_MEETS_ZERO ⪯  RA_UNIV_HALT.
+Proof.
+  apply reduces_dependent; exists.
+  intros n; exists n.
+  symmetry; apply ra_min_univ_spec.
+  apply ra_pr_univ_pr.
+Qed.
 
+Theorem PRIMEREC_PRIMESEQ_MEETS_ZERO : PRIMEREC_UNIV_MEETS_ZERO ⪯ PRIMESEQ_MEETS_ZERO.
+Proof.
+  apply reduces_dependent; exists.
+  unfold PRIMEREC_UNIV_PROBLEM, PRIMESEQ_PROBLEM.
+  intros n. 
+  exists (exist _ _ (ra_prime_seq_univ_pr _ ra_pr_univ_pr n)).
+  unfold PRIMESEQ_MEETS_ZERO, proj1_sig.
+  symmetry; apply ra_prime_seq_univ_spec.
+Qed.
+
+Theorem PRIMESEQ_NATSEQ_MEETS_ZERO : PRIMESEQ_MEETS_ZERO ⪯ NATSEQ_MEETS_ZERO.
+Proof.
+  apply reduces_dependent; exists.
+  intros (f & Hf).
+  destruct (prim_rec_reif _ Hf) as (g & Hg).
+  exists (fun n => g (n##vec_nil)).
+  unfold PRIMESEQ_MEETS_ZERO, proj1_sig, NATSEQ_MEETS_ZERO.
+  split; intros (n & Hn); exists n.
+  + revert Hn; apply ra_rel_fun; auto.
+  + rewrite <- Hn; auto.
+Qed.
 
 (* We build a similar one based on Andrej Dudenhefner
     type of H10 constraints, ie 1+x+y*y = z *)
@@ -75,5 +114,3 @@ Proof.
 Qed.
 
 Check H10UC_SAT_RA_UNIV_AD_HALT.
-
-
